@@ -1,0 +1,10 @@
+/-
+`argint` meets its specification, given `myproc` and `argraw`.
+-/
+import Xv6.ProofArgint
+
+namespace Xv6
+
+theorem Argint (MP : MYPROC) (AR : ARGRAW) : ARGINT := argint_proof MP AR
+
+end Xv6
